more aignet absstobj updates

books/centaur/aignet/aignet-logic-interface.lisp
@@ -1,6 +1,6 @@
 
 
-(in-package "AIGNET$A")
+(in-package "AIGNET")
 
 (include-book "aignet-logic")
 (local (include-book "arithmetic/top-with-meta" :dir :system))
@@ -14,252 +14,248 @@
                            acl2::make-list-ac-redef
                            sets::double-containment
                            sets::sets-are-true-lists
-                           make-list-ac
-                           acl2::duplicity-when-non-member-equal)))
+                           make-list-ac)))
 
 (local (in-theory (disable true-listp-update-nth
                            acl2::nth-with-large-index)))
 
 
-(define aignet-well-formedp (aignet)
+(define aignet$a::aignet-well-formedp (aignet)
   :enabled t
   (and (node-listp aignet)
        (aignet-nodes-ok aignet)))
 
-(define num-nodes ((aignet aignet-well-formedp))
+(define aignet$a::num-nodes ((aignet aignet$a::aignet-well-formedp))
   (+ 1 (len aignet))
   :enabled t)
 
-(define num-ins ((aignet aignet-well-formedp))
-  (duplicity :pi (tags aignet))
+(define aignet$a::num-ins ((aignet aignet$a::aignet-well-formedp))
+  (stype-count (pi-stype) aignet)
   :enabled t)
 
-(define num-regs ((aignet aignet-well-formedp))
+(define aignet$a::num-regs ((aignet aignet$a::aignet-well-formedp))
   :enabled t
-  (duplicity :ro (tags aignet)))
+  (stype-count (reg-stype) aignet))
 
-(define num-outs ((aignet aignet-well-formedp))
-  (duplicity :po (tags aignet))
+(define aignet$a::num-outs ((aignet aignet$a::aignet-well-formedp))
+  (stype-count (po-stype) aignet)
   :enabled t)
 
-(define num-regins ((aignet aignet-well-formedp))
-  (duplicity :ri (tags aignet))
+(define aignet$a::num-nxsts ((aignet aignet$a::aignet-well-formedp))
+  (stype-count (nxst-stype) aignet)
   :enabled t)
 
-(define num-gates ((aignet aignet-well-formedp))
-  (duplicity :gate (tags aignet))
+(define aignet$a::num-gates ((aignet aignet$a::aignet-well-formedp))
+  (stype-count (gate-stype) aignet)
   :enabled t)
 
-(define innum->id ((n natp)
-                   (aignet aignet-well-formedp))
-  :guard (< n (num-ins aignet))
+(define aignet$a::innum->id ((n natp)
+                             (aignet aignet$a::aignet-well-formedp))
+  :guard (< n (aignet$a::num-ins aignet))
   :returns (id idp)
   :enabled t
-  (to-id (len (lookup-pi n aignet))))
+  (to-id (len (lookup-stype n (pi-stype) aignet))))
 
-(define outnum->id ((n natp)
-                   (aignet aignet-well-formedp))
-  :guard (< n (num-outs aignet))
+(define aignet$a::outnum->id ((n natp)
+                              (aignet aignet$a::aignet-well-formedp))
+  :guard (< n (aignet$a::num-outs aignet))
   :returns (id idp)
   :enabled t
-  (to-id (len (lookup-po n aignet))))
+  (to-id (len (lookup-stype n (po-stype) aignet))))
 
-(define regnum->ro ((n natp)
-                    (aignet aignet-well-formedp))
-  :guard (< n (num-regs aignet))
+(define aignet$a::regnum->id ((n natp)
+                              (aignet aignet$a::aignet-well-formedp))
+  :guard (< n (aignet$a::num-regs aignet))
   :returns (id idp)
   :enabled t
-  (to-id (len (lookup-ro n aignet))))
+  (to-id (len (lookup-stype n (reg-stype) aignet))))
 
-(define id-existsp ((id idp) (aignet aignet-well-formedp))
+(define aignet$a::id-existsp ((id idp) (aignet aignet$a::aignet-well-formedp))
   :enabled t
   (aignet-idp id aignet))
 
-(define id->type ((id idp)
-                  (aignet aignet-well-formedp))
-  :guard (id-existsp id aignet)
+(define aignet$a::id->type ((id idp)
+                            (aignet aignet$a::aignet-well-formedp))
+  :guard (aignet$a::id-existsp id aignet)
   :enabled t
-  (node->type (car (lookup-node id aignet))))
+  (node->type (car (lookup-id id aignet))))
 
-(define io-id->regp ((id idp)
-                     (aignet aignet-well-formedp))
-  :guard (and (id-existsp id aignet)
-              (or (eql (id->type id aignet) (in-type))
-                  (eql (id->type id aignet) (out-type))))
+(define aignet$a::io-id->regp ((id idp)
+                               (aignet aignet$a::aignet-well-formedp))
+  :guard (and (aignet$a::id-existsp id aignet)
+              (or (eql (aignet$a::id->type id aignet) (in-type))
+                  (eql (aignet$a::id->type id aignet) (out-type))))
   :enabled t
-  (io-node->regp (car (lookup-node id aignet))))
+  (io-node->regp (car (lookup-id id aignet))))
 
-(define co-id->fanin ((id idp)
-                      (aignet aignet-well-formedp))
-  :guard (and (id-existsp id aignet)
-              (eql (id->type id aignet) (out-type)))
+(define aignet$a::co-id->fanin ((id idp)
+                                (aignet aignet$a::aignet-well-formedp))
+  :guard (and (aignet$a::id-existsp id aignet)
+              (eql (aignet$a::id->type id aignet) (out-type)))
   :enabled t
-  (co-node->fanin (car (lookup-node id aignet))))
+  (aignet-lit-fix
+   (co-node->fanin (car (lookup-id id aignet)))
+   (cdr (lookup-id id aignet))))
 
-(define gate-id->fanin0 ((id idp)
-                        (aignet aignet-well-formedp))
-  :guard (and (id-existsp id aignet)
-              (eql (id->type id aignet) (gate-type)))
+(define aignet$a::gate-id->fanin0 ((id idp)
+                                   (aignet aignet$a::aignet-well-formedp))
+  :guard (and (aignet$a::id-existsp id aignet)
+              (eql (aignet$a::id->type id aignet) (gate-type)))
   :enabled t
-  (gate-node->fanin0 (car (lookup-node id aignet))))
+  (aignet-lit-fix
+   (gate-node->fanin0 (car (lookup-id id aignet)))
+   (cdr (lookup-id id aignet))))
 
-(define gate-id->fanin1 ((id idp)
-                        (aignet aignet-well-formedp))
-  :guard (and (id-existsp id aignet)
-              (eql (id->type id aignet) (gate-type)))
+(define aignet$a::gate-id->fanin1 ((id idp)
+                                   (aignet aignet$a::aignet-well-formedp))
+  :guard (and (aignet$a::id-existsp id aignet)
+              (eql (aignet$a::id->type id aignet) (gate-type)))
   :enabled t
-  (gate-node->fanin1 (car (lookup-node id aignet))))
+  (aignet-lit-fix
+   (gate-node->fanin1 (car (lookup-id id aignet)))
+   (cdr (lookup-id id aignet))))
 
-(define io-id->ionum ((id idp) (aignet aignet-well-formedp))
-  :guard (and (id-existsp id aignet)
-              (or (eql (id->type id aignet) (in-type))
-                  (and (eql (id->type id aignet) (out-type))
-                       (eql (io-id->regp id aignet) 0))))
+(define aignet$a::io-id->ionum ((id idp) (aignet aignet$a::aignet-well-formedp))
+  :guard (and (aignet$a::id-existsp id aignet)
+              (or (eql (aignet$a::id->type id aignet) (in-type))
+                  (and (eql (aignet$a::id->type id aignet) (out-type))
+                       (eql (aignet$a::io-id->regp id aignet) 0))))
   :enabled t
-  (b* (((cons node rest) (lookup-node id aignet)))
-    (io-node->ionum node rest)))
+  (let ((look (lookup-id id aignet)))
+    (stype-count (stype (car look)) (cdr look)) ))
 
-(define reg-id->ri ((id idp)
-                    (aignet aignet-well-formedp))
-  :guard (and (id-existsp id aignet)
-              (eql (id->type id aignet) (in-type))
-              (eql (io-id->regp id aignet) 1))
+(define aignet$a::reg-id->nxst ((id idp)
+                              (aignet aignet$a::aignet-well-formedp))
+  :guard (and (aignet$a::id-existsp id aignet)
+              (eql (aignet$a::id->type id aignet) (in-type))
+              (eql (aignet$a::io-id->regp id aignet) 1))
   :returns (id idp)
   :enabled t
-  (to-id (len (lookup-reg->ri id aignet))))
+  (to-id (len (lookup-reg->nxst id aignet))))
 
-(define ri-id->reg ((id idp)
-                    (aignet aignet-well-formedp))
-  :guard (and (id-existsp id aignet)
-              (eql (id->type id aignet) (out-type))
-              (eql (io-id->regp id aignet) 1))
+(define aignet$a::nxst-id->reg ((id idp)
+                    (aignet aignet$a::aignet-well-formedp))
+  :guard (and (aignet$a::id-existsp id aignet)
+              (eql (aignet$a::id->type id aignet) (out-type))
+              (eql (aignet$a::io-id->regp id aignet) 1))
   :returns (id idp)
   :enabled t
-  (id-fix ;; so that the result is an ID regardless of malformed input
-   (ri-node->reg (car (lookup-node id aignet)))))
+  (aignet-id-fix ;; so that the result is an ID regardless of malformed input
+   (nxst-node->reg (car (lookup-id id aignet)))
+   (cdr (lookup-id id aignet))))
 
 
 
-(define fanout-litp ((lit litp) (aignet aignet-well-formedp))
+(define aignet$a::fanout-litp ((lit litp) (aignet aignet$a::aignet-well-formedp))
   :enabled t
   (aignet-litp lit aignet))
 
 
 
-(defsection id->phase
+(defsection aignet$a::id->phase
   (mutual-recursion
-   (defun lit->phase (lit aignet)
-     (declare (xargs :guard (and (aignet-well-formedp aignet)
+   (defun aignet$a::lit->phase (lit aignet)
+     (declare (xargs :guard (and (aignet$a::aignet-well-formedp aignet)
                                  (litp lit)
-                                 (fanout-litp lit aignet))
+                                 (aignet$a::fanout-litp lit aignet))
                      :verify-guards nil
                      :measure (acl2::two-nats-measure
                                (id-val (lit-id lit)) 1)))
      (b-xor (lit-neg lit)
-            (id->phase (lit-id lit) aignet)))
+            (aignet$a::id->phase (lit-id lit) aignet)))
 
-   (defun id->phase (id aignet)
-     (declare (Xargs :guard (and (aignet-well-formedp aignet)
+   (defun aignet$a::id->phase (id aignet)
+     (declare (Xargs :guard (and (aignet$a::aignet-well-formedp aignet)
                                  (idp id)
-                                 (id-existsp id aignet))
+                                 (aignet$a::id-existsp id aignet))
                      :measure (acl2::two-nats-measure
-                               (id-val id) 0)
-                     :hints (("goal" :in-theory (enable co-orderedp
-                                                        gate-orderedp)))))
-     (let ((type (id->type id aignet)))
+                               (id-val id) 0)))
+     (let ((type (aignet$a::id->type id aignet)))
        (cond ((eql type (out-type))
-              (if (co-orderedp id aignet)
-                  (lit->phase (co-id->fanin id aignet) aignet)
-                0))
+              (aignet$a::lit->phase (aignet$a::co-id->fanin id aignet) aignet))
              ((eql type (gate-type))
-              (if (gate-orderedp id aignet)
-                  (b-and (lit->phase (gate-id->fanin0 id aignet) aignet)
-                         (lit->phase (gate-id->fanin1 id aignet) aignet))
-                0))
+              (b-and (aignet$a::lit->phase (aignet$a::gate-id->fanin0 id aignet) aignet)
+                     (aignet$a::lit->phase (aignet$a::gate-id->fanin1 id aignet) aignet)))
              (t 0)))))
 
-  (in-theory (disable lit->phase id->phase))
+  (in-theory (disable aignet$a::lit->phase aignet$a::id->phase))
 
   (defthm bitp-of-lit->phase
-    (bitp (lit->phase lit aignet))
-    :hints (("goal" :expand (lit->phase lit aignet))))
+    (bitp (aignet$a::lit->phase lit aignet))
+    :hints (("goal" :expand (aignet$a::lit->phase lit aignet))))
 
   (defthm bitp-of-id->phase
-    (bitp (id->phase id aignet))
-    :hints (("goal" :expand (id->phase id aignet))))
+    (bitp (aignet$a::id->phase id aignet))
+    :hints (("goal" :expand (aignet$a::id->phase id aignet))))
 
-  (verify-guards id->phase)
+  (verify-guards aignet$a::id->phase)
 
-  (flag::make-flag phase-flg id->phase
-                   :hints (("goal" :in-theory (enable co-orderedp
-                                                      gate-orderedp))))
+  (flag::make-flag phase-flg aignet$a::id->phase)
 
   (defthm-phase-flg
-    (defthm id->phase-of-suffix
-      (implies (and (suffixp aignet new)
+    (defthm aignet$a::id->phase-of-suffix
+      (implies (and (aignet-extension-p new aignet)
                     (<= (id-val id) (len aignet)))
-               (equal (id->phase id new)
-                      (id->phase id aignet)))
+               (equal (aignet$a::id->phase id new)
+                      (aignet$a::id->phase id aignet)))
       :hints ('(:expand ((:free (aignet)
-                          (id->phase id aignet)))
-                :in-theory (enable gate-orderedp
-                                   co-orderedp)))
-      :flag id->phase)
-    (defthm lit->phase-of-suffix
-      (implies (and (suffixp aignet new)
+                          (aignet$a::id->phase id aignet)))))
+      :flag aignet$a::id->phase)
+    (defthm aignet$a::lit->phase-of-suffix
+      (implies (and (aignet-extension-p new aignet)
                     (<= (id-val (lit-id lit)) (len aignet)))
-               (equal (lit->phase lit new)
-                      (lit->phase lit aignet)))
+               (equal (aignet$a::lit->phase lit new)
+                      (aignet$a::lit->phase lit aignet)))
       :hints ('(:expand ((:free (aignet)
-                          (lit->phase lit aignet)))))
-      :flag lit->phase))
+                          (aignet$a::lit->phase lit aignet)))))
+      :flag aignet$a::lit->phase))
 
-  (defthm id->phase-of-cons
+  (defthm aignet$a::id->phase-of-cons
     (implies (<= (id-val id) (len aignet))
-             (equal (id->phase id (cons node aignet))
-                    (id->phase id aignet)))
-    :hints (("goal" :use ((:instance id->phase-of-suffix
+             (equal (aignet$a::id->phase id (cons node aignet))
+                    (aignet$a::id->phase id aignet)))
+    :hints (("goal" :use ((:instance aignet$a::id->phase-of-suffix
                            (new (cons node aignet))
                            (aignet aignet)))
              :expand ((:free (a b)
-                       (suffixp a (cons b a)))))))
+                       (aignet-extension-p (cons b a) a))))))
 
-  (defthm lit->phase-of-cons
+  (defthm aignet$a::lit->phase-of-cons
     (implies (<= (id-val (lit-id lit)) (len aignet))
-             (equal (lit->phase lit (cons node aignet))
-                    (lit->phase lit aignet)))
-    :hints (("goal" :use ((:instance lit->phase-of-suffix
+             (equal (aignet$a::lit->phase lit (cons node aignet))
+                    (aignet$a::lit->phase lit aignet)))
+    :hints (("goal" :use ((:instance aignet$a::lit->phase-of-suffix
                            (new (cons node aignet))
                            (aignet aignet)))
              :expand ((:free (a b)
-                       (suffixp a (cons b a))))))))
+                       (aignet-extension-p (cons b a) a)))))))
 
 
 
 
-(define aignet-add-in ((aignet aignet-well-formedp))
+(define aignet$a::aignet-add-in ((aignet aignet$a::aignet-well-formedp))
   (cons (pi-node) aignet)
   :enabled t
   ///
-  (defthm aignet-well-formedp-of-aignet-add-in
+  (defthm aignet$a::aignet-well-formedp-of-aignet-add-in
     (implies (aignet-nodes-ok aignet)
-             (aignet-nodes-ok (cons '(:pi) aignet)))
+             (aignet-nodes-ok (cons (list (pi-stype)) aignet)))
     :hints(("Goal" :in-theory (enable aignet-nodes-ok)))))
 
-(define aignet-add-reg ((aignet aignet-well-formedp))
-  (cons (ro-node) aignet)
+(define aignet$a::aignet-add-reg ((aignet aignet$a::aignet-well-formedp))
+  (cons (reg-node) aignet)
   :enabled t
   ///
   (defthm aignet-nodes-ok-of-aignet-add-reg
     (implies (aignet-nodes-ok aignet)
-             (aignet-nodes-ok (cons '(:ro) aignet)))
+             (aignet-nodes-ok (cons (list (reg-stype)) aignet)))
     :hints(("Goal" :in-theory (enable aignet-nodes-ok)))))
 
-(define aignet-add-gate ((f0 litp)
+(define aignet$a::aignet-add-gate ((f0 litp)
                          (f1 litp)
-                         (aignet aignet-well-formedp))
-  :guard (and (fanout-litp f0 aignet)
-              (fanout-litp f1 aignet))
+                         (aignet aignet$a::aignet-well-formedp))
+  :guard (and (aignet$a::fanout-litp f0 aignet)
+              (aignet$a::fanout-litp f1 aignet))
   (cons (gate-node (aignet-lit-fix f0 aignet)
                    (aignet-lit-fix f1 aignet))
         aignet)
@@ -267,53 +263,56 @@
   ///
   (defthm aignet-nodes-ok-of-aignet-add-gate
     (implies (and (aignet-nodes-ok aignet)
-                  (fanout-litp f0 aignet)
-                  (fanout-litp f1 aignet))
+                  (aignet$a::fanout-litp f0 aignet)
+                  (aignet$a::fanout-litp f1 aignet))
              (aignet-nodes-ok (cons (gate-node f0 f1) aignet)))
     :hints(("Goal" :in-theory (enable aignet-nodes-ok)))))
 
-(define aignet-add-out ((f litp)
-                        (aignet aignet-well-formedp))
-  :guard (fanout-litp f aignet)
+(define aignet$a::aignet-add-out ((f litp)
+                        (aignet aignet$a::aignet-well-formedp))
+  :guard (aignet$a::fanout-litp f aignet)
   (cons (po-node (aignet-lit-fix f aignet))
         aignet)
   :enabled t
   ///
   (defthm aignet-nodes-ok-of-aignet-add-out
     (implies (and (aignet-nodes-ok aignet)
-                  (fanout-litp f aignet))
+                  (aignet$a::fanout-litp f aignet))
              (aignet-nodes-ok (cons (po-node f) aignet)))
     :hints(("Goal" :in-theory (enable aignet-nodes-ok)))))
 
-(define aignet-add-regin ((f litp)
+(define aignet$a::aignet-set-nxst ((f litp)
                           (regid idp)
-                          (aignet aignet-well-formedp))
-  :guard (and (fanout-litp f aignet)
-              (id-existsp regid aignet)
-              (eql (id->type regid aignet) (in-type))
-              (eql (io-id->regp regid aignet) 1))
-  (cons (ri-node (aignet-lit-fix f aignet)
+                          (aignet aignet$a::aignet-well-formedp))
+  :guard (and (aignet$a::fanout-litp f aignet)
+              (aignet$a::id-existsp regid aignet)
+              (eql (aignet$a::id->type regid aignet) (in-type))
+              (eql (aignet$a::io-id->regp regid aignet) 1))
+  (cons (nxst-node (aignet-lit-fix f aignet)
                  (aignet-id-fix regid aignet))
         aignet)
   :enabled t
   ///
-  (defthm aignet-nodes-ok-of-aignet-add-regin
+  (defthm aignet-nodes-ok-of-aignet-set-nxst
     (implies (and (aignet-nodes-ok aignet)
-                  (fanout-litp f aignet)
+                  (aignet$a::fanout-litp f aignet)
                   (aignet-idp regid aignet))
-             (aignet-nodes-ok (cons (ri-node f regid) aignet)))
+             (aignet-nodes-ok (cons (nxst-node f regid) aignet)))
     :hints(("Goal" :in-theory (enable aignet-nodes-ok)))))
 
-(define aignet-clear (aignet)
+(define aignet$a::aignet-clear (aignet)
   :enabled t
   (declare (ignore aignet))
   nil)
 
-(define aignet-init ((max-outs natp)
-                     (max-regs natp)
-                     (max-ins natp)
-                     (max-nodes posp)
-                     aignet)
+(define aignet$a::aignet-init ((max-outs natp)
+                               (max-regs natp)
+                               (max-ins natp)
+                               (max-nodes posp)
+                               aignet)
   :enabled t
   (declare (ignore max-outs max-regs max-ins max-nodes aignet))
+  nil)
+
+(define aignet$a::create-aignet ()
   nil)
